Draft some actual stuff

Uppaal_Networks/AbsInt/Stack.thy
@@ -13,5 +13,44 @@ locale AbsStack = AbsWord +
   and push_correct: "c \<in> \<gamma>_stack b \<Longrightarrow> cx \<in> \<gamma>_word x \<Longrightarrow> (cx # c) \<in> \<gamma>_stack (push b x)"
   and pop_stack_correct:  "(cx # c) \<in> \<gamma>_stack b \<Longrightarrow> c \<in> \<gamma>_stack (snd (pop b))"
   and pop_return_correct: "(cx # c) \<in> \<gamma>_stack b \<Longrightarrow> cx \<in> \<gamma>_word (fst (pop b))"
+begin
+
+fun pop2 :: "'b \<Rightarrow> ('a * 'a * 'b)" where
+  "pop2 stack =
+    (let (a, astack) = pop stack;
+         (b, bstack) = pop astack
+    in (a, b, bstack))"
+lemma pop2_stack_correct: "(ca # cb # c) \<in> \<gamma>_stack b \<Longrightarrow> c \<in> \<gamma>_stack (snd (snd (pop2 b)))"
+  by (metis (no_types, lifting) Pair_inject case_prod_beta' pop2.elims pop_stack_correct prod.exhaust_sel)
+
+lemma pop2_return_b_correct: "(ca # cb # c) \<in> \<gamma>_stack b \<Longrightarrow> cb \<in> \<gamma>_word (fst (snd (pop2 b)))"
+proof -
+  assume ass: "(ca # cb # c) \<in> \<gamma>_stack b"
+  hence i: "(cb # c) \<in> \<gamma>_stack (snd (pop b))" using pop_stack_correct by simp
+  have "snd (pop2 b) = pop (snd (pop b))"
+    by (metis (no_types, lifting) case_prod_beta' pop2.elims prod.exhaust_sel snd_conv)
+  from this i show "cb \<in> \<gamma>_word (fst (snd (pop2 b)))" using pop_return_correct by auto
+qed
+
+lemma pop2_return_a_correct: "(ca # cb # c) \<in> \<gamma>_stack b \<Longrightarrow> ca \<in> \<gamma>_word (fst (pop2 b))"
+  by (metis (no_types, lifting) case_prod_beta' fst_conv pop2.elims pop_return_correct)
+
+fun pop2_push :: "('a \<Rightarrow> 'a \<Rightarrow> 'a) \<Rightarrow> 'b \<Rightarrow> 'b" where
+  "pop2_push f stack =
+    (let (a, b, rstack) = pop2 stack
+    in push rstack (f a b))"
+
+lemma[simp]: "pop2_push f stack =
+  push (snd (snd (pop2 stack))) (f (fst (pop2 stack)) (fst (snd (pop2 stack))))"
+  by (simp add: case_prod_beta)
+
+lemma pop2_push:
+  assumes
+    "\<And>x y a b. x \<in> \<gamma>_word a \<Longrightarrow> y \<in> \<gamma>_word b \<Longrightarrow> (cop x y) \<in> \<gamma>_word (f a b)"
+    "a # b # rcstack \<in> \<gamma>_stack iastack"
+  shows "(cop a b) # rcstack \<in> \<gamma>_stack (pop2_push f iastack)"
+  apply (simp add: case_prod_beta Let_def)
+  using assms by (meson pop_return_correct pop_stack_correct push_correct)
+end
 
 end
