Uppaal_Networks/AbsInt/Stack_Direct.thy
@@ -1,0 +1,87 @@
+theory Stack_Direct
+  imports Stack State_Smart
+begin
+
+type_synonym 'a stack_direct = "'a list toption"
+
+instantiation toption :: (bounded_semilattice_sup_bot) absstack
+begin
+instance ..
+end
+
+fun \<gamma>_stack_direct :: "('a \<Rightarrow> int set) \<Rightarrow> 'a stack_direct \<Rightarrow> stack set" where
+  "\<gamma>_stack_direct _ Top = \<top>" |
+  "\<gamma>_stack_direct \<gamma>_word (Minor l) = \<gamma>_list \<gamma>_word l"
+
+fun push_stack_direct :: "'a stack_direct \<Rightarrow> 'a \<Rightarrow> 'a stack_direct" where
+  "push_stack_direct Top _ = Top" |
+  "push_stack_direct (Minor l) x = Minor (x # l)"
+
+fun pop_stack_direct :: "('a::{bot, top}) stack_direct \<Rightarrow> ('a * 'a stack_direct)" where
+  "pop_stack_direct Top = (\<top>, Top)" |
+  "pop_stack_direct (Minor []) = (\<bottom>, Minor [])" |
+  "pop_stack_direct (Minor (a # as)) = (a, Minor as)"
+
+locale StackDirect = AbsStack \<gamma>_word contains make concretize aplus lt le eq "\<gamma>_stack_direct \<gamma>_word" push_stack_direct pop_stack_direct
+  for \<gamma>_word contains make concretize aplus lt le eq
+
+sublocale AbsWord \<subseteq> Direct: StackDirect
+proof(standard, goal_cases)
+  case (1 a b)
+  then show ?case
+  proof (cases b)
+    case (Minor sb)
+    from this obtain sa where sa: "a = Minor sa" using 1 less_eq_toption.elims(2) by blast
+    from this Minor show ?thesis using 1 mono_gamma_list mono_gamma by auto
+  qed simp
+next
+  case 2
+  then show ?case by simp
+next
+  case (3 c rest cx a)
+  then show ?case
+  proof (cases rest)
+    case (Minor as)
+    hence "cx # c \<in> {l. \<exists>x xs. l = x # xs \<and> x \<in> \<gamma>_word a \<and> xs \<in> \<gamma>_list \<gamma>_word as}" using 3(1) 3(2) by auto
+    then show ?thesis by (simp add: Minor)
+  qed simp
+next
+  case (4 cx c b)
+  then show ?case
+  proof (cases b)
+    case (Minor l)
+    then show ?thesis
+    proof (cases l)
+      case Nil
+      hence "\<gamma>_stack_direct \<gamma>_word b = {[]}" using Minor by simp
+      hence False using 4 by simp
+      thus ?thesis ..
+    next
+      case (Cons a as)
+      then show ?thesis using 4 Minor by auto
+    qed
+  qed simp
+next
+  case (5 cx c b)
+  then show ?case
+  proof (cases b)
+    case (Minor l)
+    then show ?thesis
+    proof (cases l)
+      case Nil
+      hence "\<gamma>_stack_direct \<gamma>_word b = {[]}" using Minor by simp
+      hence False using 5 by simp
+      thus ?thesis ..
+    next
+      case (Cons a as)
+      then show ?thesis using 5 Minor by auto
+    qed
+  qed simp
+qed
+
+context AbsWord
+begin
+abbreviation "ai_loop \<equiv> Direct.ai_loop"
+end
+
+end
