Uppaal_Networks/AbsInt/Word_Set.thy
@@ -1,0 +1,108 @@
+theory Word_Set
+  imports Word Toption State_Smart Stack_Direct
+begin
+
+datatype int_set_base = IntSet "int list"
+type_synonym int_set = "int_set_base toption"
+
+instantiation int_set_base :: bounded_semilattice_sup_bot
+begin
+instance sorry
+end
+
+instantiation toption :: (bounded_semilattice_sup_bot) absword
+begin
+instance ..
+end
+
+fun \<gamma>_int_set :: "int_set \<Rightarrow> int set" where
+  "\<gamma>_int_set Top = \<top>" |
+  "\<gamma>_int_set (Minor (IntSet v)) = set v"
+
+fun int_set_contains :: "int_set \<Rightarrow> int \<Rightarrow> bool" where
+  "int_set_contains Top _ = True" |
+  "int_set_contains (Minor (IntSet v)) x = (x \<in> set v)"
+
+fun int_set_make :: "int \<Rightarrow> int_set" where
+  "int_set_make x = Minor (IntSet [x])"
+
+fun int_set_concretize :: "int_set \<Rightarrow> int set toption" where
+  "int_set_concretize (Minor (IntSet v)) = Minor (set v)" |
+  "int_set_concretize Top = Top"
+
+fun int_set_aplus :: "int_set \<Rightarrow> int_set \<Rightarrow> int_set" where
+  "int_set_aplus (Minor (IntSet a)) (Minor (IntSet b)) = Minor (IntSet (sorted_list_of_set {x. \<exists>xa xb. x = xa + xb \<and> xa \<in> set a \<and> xb \<in> set b}))" |
+  "int_set_aplus _ _ = Top"
+
+fun int_set_lt :: "int_set \<Rightarrow> int_set \<Rightarrow> power_bool" where
+  "int_set_lt (Minor (IntSet a)) (Minor (IntSet b)) =
+    (if \<forall>xa xb. xa \<in> set a \<longrightarrow> xb \<in> set b \<longrightarrow> xa < xb
+     then BTrue
+     else if \<forall>xa xb. xa \<in> set a \<longrightarrow> xb \<in> set b \<longrightarrow> xa \<ge> xb
+     then BFalse
+     else BBoth)" |
+  "int_set_lt Top _ = BBoth" |
+  "int_set_lt _ Top = BBoth"
+
+fun int_set_le :: "int_set \<Rightarrow> int_set \<Rightarrow> power_bool" where
+  "int_set_le (Minor (IntSet a)) (Minor (IntSet b)) =
+    (if \<forall>xa xb. xa \<in> set a \<longrightarrow> xb \<in> set b \<longrightarrow> xa \<le> xb
+     then BTrue
+     else if \<forall>xa xb. xa \<in> set a \<longrightarrow> xb \<in> set b \<longrightarrow> xa > xb
+     then BFalse
+     else BBoth)" |
+  "int_set_le Top _ = BBoth" |
+  "int_set_le _ Top = BBoth"
+
+fun int_set_eq :: "int_set \<Rightarrow> int_set \<Rightarrow> power_bool" where
+  "int_set_eq (Minor (IntSet [xa])) (Minor (IntSet [xb])) = powerup (xa = xb)" |
+  "int_set_eq (Minor (IntSet a)) (Minor (IntSet b)) =
+    (if \<exists>x. x \<in> set a \<and> x \<in> set b
+     then BBoth
+     else BFalse)" |
+  "int_set_eq Top _ = BBoth" |
+  "int_set_eq _ Top = BBoth"
+
+global_interpretation WordSet: AbsWord
+  where \<gamma>_word = \<gamma>_int_set
+    and contains = int_set_contains
+    and make = int_set_make
+    and concretize = int_set_concretize
+    and aplus = int_set_aplus
+    and lt = int_set_lt
+    and le = int_set_le
+    and eq = int_set_eq
+  defines word_set_loop = WordSet.ai_loop
+proof (standard, goal_cases)
+  case (1 a b)
+  then show ?case sorry
+next
+  case 2
+  then show ?case sorry
+next
+  case (3 a x)
+  then show ?case sorry
+next
+  case (4 v)
+  then show ?case sorry
+next
+  case (5 a vs)
+  then show ?case sorry
+next
+  case (6 a vs)
+  then show ?case sorry
+next
+  case (7 x a y b)
+  then show ?case sorry
+next
+  case (8 a b)
+  then show ?case sorry
+next
+  case (9 a b)
+  then show ?case sorry
+next
+  case (10 a b)
+  then show ?case sorry
+qed
+
+end
